CellularAutomatas/proofs/causal.lean
@@ -1,0 +1,90 @@
+import CellularAutomatas.defs
+import CellularAutomatas.proofs.basic
+import Mathlib.Data.List.Basic
+
+namespace CellularAutomatas
+
+section Causal
+
+@[simp]
+lemma IsCausal.empty {α β: Type} {f: Word α → Word β} (h: IsCausal f): f [] = [] := by
+  have := (h []).1
+  simp_all
+
+@[simp]
+lemma IsCausal.comp {α β γ: Type} (f: Word α → Word β) (g: Word β → Word γ)
+    (hf: IsCausal f) (hg: IsCausal g): IsCausal (g ∘ f) := by
+  intro w
+  constructor
+  · simp only [Function.comp_apply, (hg (f w)).1, (hf w).1]
+  · intro i
+    simp only [Function.comp_apply]
+    rw [(hf w).2 i, (hg _).2 i]
+
+@[simp]
+lemma IsCausal.take_of_concat {α β: Type} {f: Word α → Word β} (h: IsCausal f) (v w: Word α):
+    (f (v ++ w))⟦*..v.length⟧ = f v := by
+  rw [← (h (v ++ w)).2 v.length]
+  simp
+
+private lemma word_getElem_eq_take_getLast {α: Type} (w: Word α) {i: ℕ} (h: i < w.length):
+    w[i] = (w.take (i + 1)).getLast (by simp; grind) := by
+  grind
+
+lemma IsCausal.eq_iff {α β: Type} (f g: Word α → Word β) (h1: IsCausal f) (h2: IsCausal g):
+  (f = g) ↔ (∀ w, (f w).getLast? = (g w).getLast?) := by
+  constructor
+  · intro h w; simp [h]
+  · intro h
+    funext w
+    apply List.ext_getElem ((h1 w).1.trans (h2 w).1.symm)
+    intro i h_len _
+    let w' := w.take (i + 1)
+    have hw' : f w' = (f w).take (i+1) := by rw [(h1 w).2]
+    have gw' : g w' = (g w).take (i+1) := by rw [(h2 w).2]
+    have h_last := h w'
+    rw [hw', gw'] at h_last
+
+    rw [word_getElem_eq_take_getLast _ h_len]
+    rw [word_getElem_eq_take_getLast _ (by rw [(h2 w).1, ←(h1 w).1]; exact h_len)]
+
+    have ne_nil : (f w).take (i+1) ≠ [] := by
+      apply List.ne_nil_of_length_pos
+      rw [List.length_take]
+      have : i < (f w).length := h_len
+      omega
+
+    have ne_nil_g : (g w).take (i+1) ≠ [] := by
+      apply List.ne_nil_of_length_pos
+      rw [List.length_take]
+      rw [(h2 w).1, ←(h1 w).1]
+      have : i < (f w).length := h_len
+      omega
+
+    rw [List.getLast?_eq_getLast_of_ne_nil ne_nil, List.getLast?_eq_getLast_of_ne_nil ne_nil_g] at h_last
+    simp_all
+
+@[simp]
+lemma CellAutomaton.trace_rt_is_causal {α β: Type} [Alphabet α] [Alphabet β] (C: CellAutomaton α？ β): IsCausal C.trace_rt := by
+  intro w
+  constructor
+  · apply trace_rt_len
+  · intro i
+    let p := w.take i
+    let s := w.drop i
+    conv =>
+      rhs
+      rw [(List.take_append_drop i w).symm]
+    change C.trace_rt p = (C.trace_rt (p ++ s)).take i
+    rw [←LCellAutomaton.scan_temporal_independence C p s]
+    apply List.ext_getElem
+    · simp only [trace_rt_len, p, s, List.length_take, List.length_drop, List.length_append]
+      omega
+    · intro j h1 h2
+      simp only [List.getElem_take]
+
+lemma Advice.causal_iff {α Γ: Type} (adv: Advice α Γ): adv.causal ↔ IsCausal adv.f := by rfl
+
+end Causal
+
+end CellularAutomatas
